src/QueryStructure/Refinements/GeneralQueryRefinements.v
@@ -5,7 +5,7 @@ Require Import String List Sorting.Permutation
         EnsembleListEquivalence.
 
 (* [Query_For] and all aggregates are opaque, so we need to make them
-   transparent in order to reason about them. *) 
+   transparent in order to reason about them. *)
 Local Transparent Query_For Count Max MaxN MaxZ Sum SumN SumZ.
 Require Import NArith ZArith.
 
@@ -220,11 +220,6 @@ Lemma DropQSConstraintsQuery_In_UnderBinder {A B} :
 Proof.
   reflexivity.
 Qed.
-
-Definition UnIndexedEnsembleListEquivalence
-           {heading} R (l : list (@Tuple heading))  :=
-  exists l', (map indexedTuple l') = l /\
-  EnsembleListEquivalence R l'.
 
 (*Lemma Equivalent_Swap_In {ResultT}
       qsSchema qs R (bod : Tuple -> Comp (list ResultT))
