examples/BookstoreSemiAutomatic.v
@@ -57,18 +57,23 @@ Definition BookStoreSig : ADTSig :=
   ADTsignature {
       "Init" : unit → rep,
       "PlaceOrder" : rep × Order → rep × bool,
+      "DeleteOrder" : rep × nat → rep × list Order,
       "AddBook" : rep × Book → rep × bool,
       "GetTitles" : rep × string → rep × list string,
       "NumOrders" : rep × string → rep × nat
     }.
 
 (* Now we write what the methods should actually do. *)
+
 Definition BookStoreSpec : ADT BookStoreSig :=
   QueryADTRep BookStoreSchema {
     const "Init" (_ : unit) : rep := empty,
 
     update "PlaceOrder" ( o : Order ) : bool :=
         Insert o into sORDERS,
+
+    update "DeleteOrder" ( oid : nat ) : list Order :=
+        Delete o from sORDERS where o!sISBN = oid ,
 
     update "AddBook" ( b : Book ) : bool :=
         Insert b into sBOOKS ,
@@ -118,6 +123,8 @@ Definition BookStore_AbsR
            (or : UnConstrQueryStructure BookStoreSchema)
            (nr : TBookStorage * TOrderStorage) : Prop :=
   or!sBOOKS ≃ fst nr /\ or!sORDERS ≃ snd nr.
+
+Opaque QSDelete.
 
 Definition BookStoreManual :
   Sharpened BookStoreSpec.
@@ -238,6 +245,7 @@ Proof.
        checks failed. *)
     Split Constraint Checks.
 
+    (* First, the case where checks succeed: the insertion is valid: *)
     checksSucceeded.
 
     (* Second, the case where checks failed: in that case, the DB
@@ -297,6 +305,439 @@ Proof.
   hone method "NumOrders". {
     observer.
   }
+
+  hone method "DeleteOrder". {
+    startMethod BookStore_AbsR.
+
+    Lemma EnsembleComplementIntersection {A}
+    : forall (E P : Ensemble A),
+        DecideableEnsemble P
+        -> forall (a : A),
+             (In _ (Intersection _ E
+                                (Complement _ (EnsembleDelete E P))) a
+             <-> In _ (Intersection _ E P) a).
+    Proof.
+      unfold EnsembleDelete, Complement, In in *; intuition;
+      destruct H; constructor; eauto; unfold In in *.
+      - case_eq (GeneralQueryRefinements.dec x); intros.
+        + eapply dec_decides_P; eauto.
+        + exfalso; apply H0; constructor; unfold In; eauto.
+        intros H'; apply dec_decides_P in H'; congruence.
+      - intros H'; destruct H'; unfold In in *; eauto.
+    Qed.
+
+    Global Instance IndexedDecideableEnsemble
+           {heading}
+           {P : Ensemble (@Tuple heading)}
+           {P_dec : DecideableEnsemble P}
+    : DecideableEnsemble (fun x : IndexedTuple => P x) :=
+      {| dec := @GeneralQueryRefinements.dec _ _ P_dec |}.
+    Proof.
+      intuition; eapply dec_decides_P; simpl in *; eauto.
+    Defined.
+
+    Lemma DeletedTuplesIntersection {qsSchema}
+    : forall (qs : UnConstrQueryStructure qsSchema)
+             (Ridx : @BoundedString (map relName (qschemaSchemas qsSchema)))
+             (P : Ensemble Tuple),
+        DecideableEnsemble P
+        -> refine {x | QSDeletedTuples qs Ridx P x}
+                  {x | UnIndexedEnsembleListEquivalence
+                         (Intersection _ (GetUnConstrRelation qs Ridx) P) x}.
+    Proof.
+      intros qs Ridx P P_dec v Comp_v; inversion_by computes_to_inv.
+      constructor.
+      unfold QSDeletedTuples, UnIndexedEnsembleListEquivalence in *; destruct_ex;
+        intuition; subst.
+        eexists; intuition.
+        unfold EnsembleListEquivalence in *; intuition; eauto with typeclass_instances.
+        + eapply H0; eapply EnsembleComplementIntersection; eauto with typeclass_instances.
+        + eapply EnsembleComplementIntersection; eauto with typeclass_instances.
+          eapply H0; eauto.
+    Qed.
+
+    Lemma NoDupFilter {A}
+    : forall (f : A -> bool) (l : list A),
+        NoDup l -> NoDup (filter f l).
+    Proof.
+      induction l; simpl; intros; eauto.
+      inversion H; subst; find_if_inside; try constructor; eauto.
+      unfold not; intros H'; apply H2; revert H'; clear; induction l;
+      simpl; eauto; find_if_inside; simpl; intuition.
+    Qed.
+
+    Local Transparent Query_For.
+
+    Require Import AdditionalPermutationLemmas.
+
+    Lemma DeletedTuplesFor {qsSchema}
+    : forall (qs : UnConstrQueryStructure qsSchema)
+             (Ridx : @BoundedString (map relName (qschemaSchemas qsSchema)))
+             (P : Ensemble Tuple),
+        DecideableEnsemble P
+        -> refine {x | QSDeletedTuples qs Ridx P x}
+                  (For (UnConstrQuery_In qs Ridx
+                                        (fun tup => Where (P tup) Return tup))).
+    Proof.
+      intros qs Ridx P P_dec v Comp_v; rewrite DeletedTuplesIntersection by auto.
+      constructor.
+      unfold UnIndexedEnsembleListEquivalence.
+      unfold Query_For in *; apply computes_to_inv in Comp_v; simpl in *;
+      destruct Comp_v as [l [Comp_v Perm_l_v]].
+      unfold UnConstrQuery_In, QueryResultComp in *; inversion_by computes_to_inv.
+      remember (GetUnConstrRelation qs Ridx); clear Hequ.
+      revert P_dec u v l Perm_l_v H1 H0; clear; induction x; simpl; intros.
+      - inversion_by computes_to_inv; subst.
+        exists (@nil (@IndexedTuple
+                        (schemaHeading
+                           (relSchema
+                              (@nth_Bounded NamedSchema string relName
+                                            (qschemaSchemas qsSchema) Ridx)))));
+          simpl; split; eauto.
+        rewrite Permutation_nil by eauto; reflexivity.
+        + unfold EnsembleListEquivalence in *; intuition.
+          destruct H0; eapply H1; eauto.
+      - inversion_by computes_to_inv; subst.
+        unfold UnConstrRelation in u.
+        case_eq (@GeneralQueryRefinements.dec _ P P_dec a); intros.
+        + apply computes_to_inv in H1; simpl in *; intuition.
+          apply dec_decides_P in H; apply H3 in H.
+          apply computes_to_inv in H; simpl in *; subst; simpl in *.
+          pose proof (PermutationConsSplit _ _ _ Perm_l_v); destruct_ex; subst.
+          destruct (H1 (fun x => u x /\ x <> a) (app x0 x2) x1); intuition eauto.
+          * eapply Permutation_cons_inv; rewrite Permutation_middle; eassumption.
+          * unfold EnsembleListEquivalence in *; intuition.
+            inversion H; subst; eauto.
+            unfold In in *; intuition.
+            apply H5 in H6; destruct H6; subst; eauto; congruence.
+            unfold In; intuition.
+            apply H5; simpl; intuition.
+            inversion H; subst; eauto.
+          * symmetry in H5; pose proof (app_map_inv _ _ _ _ H5); destruct_ex;
+            intuition; subst.
+            exists (app x4 (a :: x5)); simpl; rewrite map_app; intuition.
+            { unfold EnsembleListEquivalence in *; intuition.
+              - apply NoDup_app_swap; simpl; constructor; eauto.
+                inversion H; subst; unfold not; intros; apply H10.
+                assert (List.In a (x4 ++ x5)) as In_a by
+                    (apply in_or_app; apply in_app_or in H6; intuition).
+                apply H8 in In_a; destruct In_a; unfold In in *; intuition.
+                apply H7 in H13; simpl in H13; intuition.
+                + apply NoDup_app_swap; eauto.
+              - destruct H6; unfold In in *; apply H7 in H6; simpl in *; intuition.
+                apply in_or_app; simpl; intuition.
+                assert (u x0) as u_x0 by (apply H7; eauto).
+                assert (List.In x0 (x4 ++ x5)) as In_x0
+                by (apply H8; constructor; unfold In; intuition; subst;
+                    inversion H; subst; eauto).
+                apply in_or_app; simpl; apply in_app_or in In_x0; intuition.
+              - unfold In.
+                assert (List.In x0 (x4 ++ x5) \/ x0 = a)
+                  as In_x0
+                    by (apply in_app_or in H6; simpl in H6; intuition).
+                intuition.
+                apply H8 in H9; destruct H9; unfold In in *; intuition.
+                constructor; eauto.
+                subst; constructor; eauto.
+                apply H7; simpl; eauto.
+                case_eq (@GeneralQueryRefinements.dec _ P P_dec a); intros.
+                apply dec_decides_P; eauto.
+                assert (~ P a) as H''
+                                  by (unfold not; intros H'; apply dec_decides_P in H'; congruence);
+                    apply H4 in H''; discriminate.
+            }
+        + apply computes_to_inv in H1; simpl in *; intuition.
+          assert (~ P a) as H''
+                           by (unfold not; intros H'; apply dec_decides_P in H'; congruence);
+            apply H4 in H''; subst.
+          destruct (H1 (fun x => u x /\ x <> a) v x1); intuition eauto.
+          * unfold EnsembleListEquivalence in *; intuition.
+            inversion H5; subst; eauto.
+            destruct H0; apply H6 in H0; simpl in H0; intuition.
+            simpl in H6; constructor.
+            apply H6; eauto.
+            inversion H5; intros; subst; eauto.
+          * eexists; split; eauto.
+            unfold EnsembleListEquivalence in *; intuition.
+            destruct H7; intuition.
+            eapply H9; constructor; unfold In in *; subst; intuition.
+            subst; apply_in_hyp dec_decides_P; congruence.
+            constructor;
+              apply H9 in H7; destruct H7; unfold In in *; intuition.
+    Qed.
+
+    Opaque Query_For.
+
+    unfold QSDeletedTuples.
+    pose proof (@DeletedTuplesFor _ or ``(sORDERS) (fun o : Tuple => o!sISBN = n)) as H';
+    rewrite H' by eauto with typeclass_instances.
+    concretize.
+    asPerm (BookStorage, OrderStorage).
+    commit.
+    setoid_rewrite refineEquiv_pick_pair; simplify with monad laws.
+    rewrite refine_pick_val by
+        refine_bag_update_other_table.
+    simplify with monad laws.
+
+    Lemma bdelete_correct_DB
+          db_schema qs index
+          (bag_plus : BagPlusProof (@Tuple (@QSGetNRelSchemaHeading db_schema index)))
+    :  forall (store: BagTypePlus bag_plus),
+         GetUnConstrRelation qs index ≃ store
+         -> forall (DeletedTuples : Ensemble (@Tuple (@QSGetNRelSchemaHeading db_schema index)))
+                   (DT_Dec : DecideableEnsemble DeletedTuples),
+              EnsembleIndexedListEquivalence
+                (GetUnConstrRelation
+                   (@UpdateUnConstrRelation db_schema qs index
+                                            (EnsembleDelete (GetUnConstrRelation qs index)
+                                                            DeletedTuples)) index)
+                (snd (List.partition (@GeneralQueryRefinements.dec _ _ DT_Dec)
+                                     (benumerate store))).
+    Proof.
+      simpl; unfold EnsembleDelete, EnsembleBagEquivalence, In, Complement; simpl;
+      unfold EnsembleIndexedListEquivalence, UnIndexedEnsembleListEquivalence,
+      EnsembleListEquivalence; intros; intuition; destruct_ex; intuition; subst.
+      repeat setoid_rewrite get_update_unconstr_eq; simpl; intros.
+      exists x0.
+      unfold UnConstrFreshIdx in *; intros; apply H; destruct H3; eauto.
+      exists (snd (partition (@GeneralQueryRefinements.dec IndexedTuple (fun t => DeletedTuples t) _ ) x)); intuition.
+      - unfold BagPlusProofAsBag; rewrite <- H2.
+        repeat rewrite partition_filter_neq.
+        clear; induction x; simpl; eauto.
+        find_if_inside; simpl; eauto; rewrite <- IHx; reflexivity.
+      - revert H0; clear; induction x; simpl; eauto.
+        intros; inversion H0; subst.
+        case_eq (partition (fun x0 => @GeneralQueryRefinements.dec IndexedTuple (fun t => DeletedTuples t) _ x0) x); intros; simpl in *; rewrite H.
+        rewrite H in IHx; apply IHx in H3;
+        case_eq (@GeneralQueryRefinements.dec IndexedTuple (fun t => DeletedTuples t) _ a);
+        intros; simpl in *; rewrite H1; simpl; eauto.
+        constructor; eauto.
+        unfold not; intros; apply H2; eapply In_partition with
+        (f := fun x0 : IndexedTuple => @GeneralQueryRefinements.dec IndexedTuple (fun t => DeletedTuples t) _ x0).
+        simpl in *; rewrite H; eauto.
+      - rewrite get_update_unconstr_eq in H3.
+        destruct H3; unfold In in *.
+        apply H4 in H3; eapply In_partition in H3; intuition; try apply H6.
+        apply In_partition_matched in H6; apply dec_decides_P in H6; exfalso; eauto.
+      - rewrite get_update_unconstr_eq; constructor.
+        eapply H4; eapply In_partition; eauto.
+        unfold In; intros.
+        apply In_partition_unmatched in H3.
+        simpl in *; apply dec_decides_P in H5.
+        unfold QSGetNRelSchemaHeading, GetNRelSchemaHeading, GetNRelSchema in *;
+          rewrite H3 in H5; congruence.
+    Qed.
+
+    Lemma bdeletePlus_correct_DB
+          db_schema qs index
+          bag_plus
+    :  forall (store: BagTypePlus bag_plus),
+         EnsembleBagEquivalence bag_plus (GetUnConstrRelation qs index) store
+         -> forall (DeletedTuples : Ensemble (@Tuple (@QSGetNRelSchemaHeading db_schema index)))
+                   (DT_Dec : DecideableEnsemble DeletedTuples)
+                   search_term,
+              ExtensionalEq (@GeneralQueryRefinements.dec _ _ DT_Dec)
+                            (bfind_matcher (Bag := BagPlus bag_plus) search_term)     
+              -> EnsembleBagEquivalence
+                bag_plus
+                (GetUnConstrRelation
+                   (@UpdateUnConstrRelation db_schema qs index
+                                            (EnsembleDelete (GetUnConstrRelation qs index)
+                                                            DeletedTuples)) index)
+                (snd (bdelete store search_term)).
+    Proof.
+      intros; unfold ExtensionalEq, EnsembleBagEquivalence in *.
+      unfold EnsembleBagEquivalence.
+      repeat rewrite get_update_unconstr_eq; simpl; intros.
+      split;
+        [
+        | eapply bdelete_RepInv; intuition ].
+      simpl in *;
+        unfold EnsembleListEquivalence, EnsembleIndexedListEquivalence,
+        UnConstrFreshIdx, EnsembleDelete, Complement in *; intuition; destruct_ex; intuition; intros.
+      exists x; intros; eapply H; destruct H1; unfold In in *; eauto.
+      unfold UnIndexedEnsembleListEquivalence, EnsembleListEquivalence in *.
+      generalize (bdelete_correct store search_term H2); destruct_ex; intuition.
+      rewrite partition_filter_neq in H1.
+      unfold BagPlusProofAsBag in *; simpl in *; rewrite <- H4 in H1.
+      clear H6 H H2 H4.
+      remember (filter (fun a : Tuple => negb (bfind_matcher search_term a))
+            (map indexedTuple x0)).
+      revert H1 H0 x0 Heql H3 H7; clear; intro;
+      induction (benumerate (snd (bdelete store search_term))); intros.
+      - rewrite Permutation_nil in Heql; subst; eauto.
+    Admitted.
+(*      - destruct x0; simpl in *; try discriminate.
+        eexists; intuition eauto.
+        simpl; auto.
+        destruct H; eapply H7; eauto.
+        destruct H.
+        find_if_inside; try discriminate.
+      destruct_ex *)
+    simpl.
+    rewrite refine_pick_val.
+    Focus 2.
+    simpl.
+    eapply (@bdeletePlus_correct_DB _ _ _ _ _ H2 (fun x => (x!sISBN)%Tuple = n) _ (Some n, [])).
+    unfold ExtensionalEq; simpl.
+    intros; rewrite andb_true_r.
+    reflexivity.
+    simplify with monad laws.
+
+    (* Almost done!*)
+
+    unfold cast, eq_rect, eq_rect_r, eq_rect, eq_sym.
+    unfold NatTreeBag.KeyFilter, NatTreeBag.MoreFacts.BasicProperties.F.eq_dec.
+
+    simpl.
+    intros; destruct (eq_nat_dec (a!sISBN) n).
+    simpl.
+
+    simplify with monad laws.
+        (eapply bdeletePlus_correct_DB).
+    rewrite pick_val.
+
+
+
+      split.
+      Print TSearchTermMatcher.
+
+snd (List.partition (@GeneralQueryRefinements.dec _ _ DT_Dec)
+                                     (benumerate store))).
+    Proof.
+      simpl; intros; constructor.
+      - eapply bdelete_correct_DB; eauto.
+      - eapply binsert_RepInv; apply H.
+    Qed.
+
+    idtac.
+
+        simpl in *.
+pose proof (In_partition_unmatched _ _ H3); constructor.
+        elimtype False; apply H5.
+        t
+        right
+
+
+
+        find_if_inside;
+        case_eq (partition (@GeneralQueryRefinements.dec IndexedTuple _ _) x). partition_filter_neq
+        split.
+
+      simpl.
+      exists (snd
+      destruct_ex.
+      idtac.
+      simpl in H0.
+      setoid_rewrite NoDup_modulo_permutation.
+      split; intros.
+
+      rewrite
+
+    Permutation (benumerate (snd (bdelete container search_term)))
+                (snd (List.partition (bfind_matcher search_term)
+                                     (benumerate container)))
+
+
+    Lemma
+
+      {b : TOrderStorage |
+       EnsembleBagEquivalence OrderStorage
+                              ((UpdateUnConstrRelation or ``(sORDERS)
+                                                       (EnsembleDelete or!sORDERS
+                     (fun x : IndexedTuple => (x!sISBN)%Tuple = n)))!sORDERS)%QueryImpl
+              b}
+
+    setoid_rewrite refineEquiv_pick_pair.
+
+
+    setoid_rewrite refine_pick_val by
+                     (refine_bag_insert_in_other_table).
+                    || binsert_correct_DB);
+
+
+    Lemma EnsembleIntersectionFor {A}
+    : forall (E P : Ensemble A),
+        DecideableEnsemble P
+        -> forall (a : A),
+             (In _ (Intersection _ E
+                                (Complement _ (EnsembleDelete E P))) a
+             <-> In _ (Intersection _ E P) a).
+    Proof.
+      unfold EnsembleDelete, Complement, In in *; intuition;
+      destruct H; constructor; eauto; unfold In in *.
+      - case_eq (GeneralQueryRefinements.dec x); intros.
+        + eapply dec_decides_P; eauto.
+        + exfalso; apply H0; constructor; unfold In; eauto.
+        intros H'; apply dec_decides_P in H'; congruence.
+      - intros H'; destruct H'; unfold In in *; eauto.
+    Qed.
+
+
+
+    Show.
+
+    rewrite DeletedTuplesIntersection; eauto with typeclass_instances.
+
+
+Lemma binsert_correct_DB
+      db_schema qs index
+      (bag_plus : BagPlusProof (@Tuple (@QSGetNRelSchemaHeading db_schema index)))
+:  forall (store: BagTypePlus bag_plus),
+     GetUnConstrRelation qs index ≃ store
+     -> forall DeletedTuples,
+      UnIndexedEnsembleListEquivalence
+        (GetUnConstrRelation
+           (@UpdateUnConstrRelation db_schema qs index
+                                   (EnsembleDelete index DeletedTuples)) index)
+        (benumerate (bdelete (Bag := BagPlus bag_plus) store tuple)).
+Proof.
+  intros * store_eqv; destruct store_eqv as (store_eqv, store_WF).
+  unfold EnsembleIndexedTreeEquivalence_AbsR,
+  EnsembleBagEquivalence, UnIndexedEnsembleListEquivalence,
+  UnIndexedEnsembleListEquivalence, EnsembleListEquivalence in *.
+
+  setoid_rewrite get_update_unconstr_eq.
+  setoid_rewrite in_ensemble_insert_iff.
+  setoid_rewrite NoDup_modulo_permutation.
+  split; intros.
+
+  erewrite binsert_enumerate_length by eauto with typeclass_instances.
+    intuition; subst;
+    [ | apply lt_S];
+    intuition.
+
+  destruct store_eqv as (indices & [ l' (map & nodup & equiv) ]); eauto.
+
+  destruct store_eqv as (indices & [ l' (map & nodup & equiv) ]); eauto.
+
+  destruct (permutation_map_cons indexedTuple (binsert_enumerate tuple store store_WF)
+                                 {| tupleIndex := Datatypes.length (benumerate store);
+                                    indexedTuple := tuple |} l' eq_refl map)
+    as [ l'0 (map' & perm) ].
+
+  exists l'0.
+  split; [ assumption | split ].
+
+  eexists; split; try apply perm.
+
+  constructor;
+    [ rewrite <- equiv; intro abs;
+      apply indices in abs; simpl in abs;
+      eapply lt_refl_False; eauto | assumption ].
+
+  setoid_rewrite perm.
+  setoid_rewrite equiv.
+  setoid_rewrite eq_sym_iff at 1.
+  reflexivity.
+Qed.
+
+
+
+  }
+
+
+
   unfold cast, eq_rect_r, eq_rect, eq_sym; simpl.
 
   (* At this point our implementation is fully computational: we're done! *)
