src/QueryStructure/Refinements/GeneralDeleteRefinements.v
@@ -1,0 +1,546 @@
+Require Import String Omega List FunctionalExtensionality Ensembles
+        Computation ADT ADTRefinement ADTNotation QueryStructureSchema
+        BuildADTRefinements QueryStructure EnsembleListEquivalence
+        QuerySpecs.QueryQSSpecs QuerySpecs.DeleteQSSpecs
+        ConstraintChecksRefinements ListQueryStructureRefinements.
+
+(* Facts about implements delete operations. *)
+
+Section DeleteRefinements.
+
+  Hint Resolve AC_eq_nth_In AC_eq_nth_NIn crossConstr.
+  Hint Unfold SatisfiesCrossRelationConstraints
+       SatisfiesSchemaConstraints.
+
+  Arguments GetUnConstrRelation : simpl never.
+  Arguments UpdateUnConstrRelation : simpl never.
+  Arguments replace_BoundedIndex : simpl never.
+  Arguments BuildQueryStructureConstraints : simpl never.
+  Arguments BuildQueryStructureConstraints' : simpl never.
+
+  Program
+    Definition Delete_Valid
+    (qsSchema : QueryStructureSchema)
+    (qs : QueryStructure qsSchema)
+    (Ridx : _)
+    (DeletedTuples :
+       Ensemble (@Tuple (schemaHeading (QSGetNRelSchema _ Ridx))))
+    (schConstr :
+       forall tup tup',
+         EnsembleDelete (GetRelation qs Ridx) DeletedTuples tup
+         -> EnsembleDelete (GetRelation qs Ridx) DeletedTuples tup'
+         -> SatisfiesSchemaConstraints Ridx tup tup')
+   (* And is compatible with the cross-schema constraints. *)
+    (crossConstr' :
+       forall Ridx',
+         Ridx' <> Ridx ->
+        forall tup',
+          (GetRelation qs Ridx') tup'
+          -> SatisfiesCrossRelationConstraints
+               Ridx' Ridx tup'
+               (EnsembleDelete (GetRelation qs Ridx) DeletedTuples))
+  : QueryStructure qsSchema :=
+    {| rels :=
+         UpdateRelation _ (rels qs) Ridx {| rel := EnsembleDelete (GetRelation qs Ridx) DeletedTuples|}
+    |}.
+  Next Obligation.
+    unfold GetRelation.
+    unfold SatisfiesSchemaConstraints, QSGetNRelSchema, GetNRelSchema,
+    GetRelation in *.
+    set ((ith_Bounded _ (rels qs) Ridx )) as X in *; destruct X; simpl in *.
+    destruct (schemaConstraints
+                (relSchema (nth_Bounded relName (qschemaSchemas qsSchema) Ridx))); eauto.
+  Defined.
+  Next Obligation.
+    caseEq (BuildQueryStructureConstraints qsSchema idx idx'); eauto.
+    unfold SatisfiesCrossRelationConstraints, UpdateRelation in *;
+    destruct (BoundedString_eq_dec Ridx idx'); subst.
+
+    - rewrite ith_replace_BoundIndex_eq; simpl.
+      rewrite ith_replace_BoundIndex_neq in H1; eauto using string_dec.
+      generalize (crossConstr' idx H0 _ H1); rewrite H; eauto.
+    - rewrite ith_replace_BoundIndex_neq in *; eauto using string_dec.
+      destruct (BoundedString_eq_dec Ridx idx); subst.
+      + rewrite ith_replace_BoundIndex_eq in H1; simpl in *; eauto.
+        unfold EnsembleDelete in H1; destruct H1; subst; eauto.
+        * pose proof (crossConstr qs idx idx') as X; rewrite H in X; eauto.
+      + rewrite ith_replace_BoundIndex_neq in H1; eauto using string_dec.
+        pose proof (crossConstr qs idx idx') as X; rewrite H in X; eauto.
+  Qed.
+
+  Lemma QSDeleteSpec_refine :
+    forall qsSchema (qs : QueryStructure qsSchema) Ridx
+           (DeletedTuples :
+              Ensemble (@Tuple (schemaHeading (QSGetNRelSchema _ Ridx)))),
+      refine
+        (Pick (QSDeleteSpec {| qsHint := qs |} Ridx DeletedTuples))
+        (schConstr <- {b |
+                       decides
+                         b
+                         (forall tup tup',
+                            EnsembleDelete (GetRelation qs Ridx) DeletedTuples tup
+                            -> EnsembleDelete (GetRelation qs Ridx) DeletedTuples tup'
+                            -> SatisfiesSchemaConstraints Ridx tup tup')
+                      };
+            crossConstr <- {b |
+                            decides
+                              b
+                              (forall Ridx',
+                                 Ridx' <> Ridx ->
+                                 forall tup',
+                                   (GetRelation qs Ridx') tup'
+                                   -> SatisfiesCrossRelationConstraints
+                                        Ridx' Ridx tup'
+                                        (EnsembleDelete (GetRelation qs Ridx) DeletedTuples))
+                           };
+            match schConstr, crossConstr with
+              | true, true =>
+                {qs' |
+                 (forall Ridx',
+                    Ridx <> Ridx' ->
+                    GetRelation qsHint Ridx' =
+                    GetRelation qs' Ridx')
+                 /\ forall t,
+                      GetRelation qs' Ridx t <->
+                      (EnsembleDelete (GetRelation qsHint Ridx) DeletedTuples t)
+             }
+
+              | _, _ => ret qsHint
+            end).
+  Proof.
+    intros qsSchema qs Ridx DeletedTuples v Comp_v.
+    do 2 (apply_in_hyp computes_to_inv; destruct_ex; split_and).
+    destruct x; destruct x0;
+    repeat (apply_in_hyp computes_to_inv; destruct_ex; split_and); simpl in * ;
+    solve
+        [econstructor; unfold QSDeleteSpec; eauto; right; subst; intuition ].
+  Qed.
+
+  Lemma ComplementIntersection {A} :
+    forall (ens : Ensemble A) (a : A),
+      ~ In _ (Intersection A ens (Complement A ens)) a.
+  Proof.
+    unfold In, not; intros; inversion H; subst.
+    unfold Complement, In in *; tauto.
+  Qed.
+
+  Corollary ComplementIntersectionIndexedList {heading}
+  : forall (ens : Ensemble (@IndexedTuple heading)),
+      UnIndexedEnsembleListEquivalence
+        (Intersection IndexedTuple ens
+                      (Complement IndexedTuple ens))
+        [].
+  Proof.
+    unfold UnIndexedEnsembleListEquivalence.
+    exists (@nil (@IndexedTuple heading)); simpl; intuition.
+    unfold EnsembleListEquivalence.EnsembleListEquivalence; intuition.
+    - constructor.
+    - exfalso; eapply ComplementIntersection; eauto.
+  Qed.
+
+  Lemma QSDeleteSpec_UnConstr_refine' :
+    forall qsSchema (qs : UnConstrQueryStructure qsSchema)
+           (Ridx : @BoundedString (map relName (qschemaSchemas qsSchema)))
+           (or : QueryStructure qsSchema)
+           DeletedTuples,
+      DropQSConstraints_AbsR or qs ->
+      refine
+        (or' <- (qs'       <- Pick (QSDeleteSpec {|qsHint := or |} Ridx DeletedTuples);
+                 deleted   <- Pick (UnIndexedEnsembleListEquivalence
+                                      (Intersection _
+                                                    (GetRelation or Ridx)
+                                                    (Complement _ (GetRelation qs' Ridx))));
+                 ret (qs', deleted));
+         nr' <- {nr' | DropQSConstraints_AbsR (fst or') nr'};
+         ret (nr', snd or'))
+        (schConstr <- {b |
+                       decides
+                         b
+                         (forall tup tup',
+                            EnsembleDelete (GetUnConstrRelation qs Ridx) DeletedTuples tup
+                            -> EnsembleDelete (GetUnConstrRelation qs Ridx) DeletedTuples tup'
+                            -> SatisfiesSchemaConstraints Ridx tup tup')
+                      };
+            crossConstr <- (@Iterate_Decide_Comp _
+                                (fun Ridx' =>
+                                   Ridx' <> Ridx ->
+                                   forall tup',
+                                     (GetUnConstrRelation qs Ridx') tup'
+                                     -> SatisfiesCrossRelationConstraints
+                                        Ridx' Ridx tup'
+                                        (EnsembleDelete (GetUnConstrRelation qs Ridx) DeletedTuples)));
+            match schConstr, crossConstr with
+              | true, true =>
+                deleted   <- Pick (UnIndexedEnsembleListEquivalence
+                                     (Intersection _
+                                                   (GetUnConstrRelation qs Ridx)
+                                                   (Complement _ (EnsembleDelete (GetUnConstrRelation qs Ridx) DeletedTuples))));
+
+              ret (UpdateUnConstrRelation qs Ridx (EnsembleDelete (GetUnConstrRelation qs Ridx) DeletedTuples), deleted)
+              | _, _ => ret (qs, [])
+            end).
+  Proof.
+    intros.
+    setoid_rewrite refineEquiv_pick_eq'.
+    unfold DropQSConstraints_AbsR in *; intros; subst.
+    rewrite QSDeleteSpec_refine.
+    unfold refine; intros; subst.
+      do 2 (apply_in_hyp computes_to_inv; destruct_ex; split_and).
+      repeat rewrite GetRelDropConstraints in *.
+      (* These assert are gross. Need to eliminate them. *)
+      assert (
+          (fun Ridx' : BoundedIndex (map relName (qschemaSchemas qsSchema)) =>
+             Ridx' <> Ridx ->
+             forall tup' : IndexedTuple,
+               GetUnConstrRelation (DropQSConstraints or) Ridx' tup' ->
+               SatisfiesCrossRelationConstraints Ridx' Ridx tup'
+                                                 (EnsembleDelete (GetRelation or Ridx) DeletedTuples))
+          = fun Ridx' : BoundedIndex (map relName (qschemaSchemas qsSchema)) =>
+              Ridx' <> Ridx ->
+              forall tup' : IndexedTuple,
+                GetRelation or Ridx' tup' ->
+                SatisfiesCrossRelationConstraints Ridx' Ridx tup'
+                                                  (EnsembleDelete (GetRelation or Ridx) DeletedTuples))
+        as rewriteSat
+          by (apply functional_extensionality; intros; repeat rewrite GetRelDropConstraints;
+              reflexivity); rewrite rewriteSat in H1; clear rewriteSat.
+      (* Resume not-terribleness *)
+      generalize (Iterate_Decide_Comp_BoundedIndex _ _ _ H1) as H1'; intros.
+      simpl in *; revert H1.
+      repeat apply_in_hyp computes_to_inv; destruct_ex;
+      intuition; apply_in_hyp computes_to_inv; subst.
+      econstructor 2 with
+      (comp_a_value := match x as x', x0 as x0'
+                             return decides x' _ ->
+                                    decides x0' _  -> _
+                       with
+                          | true, true =>
+                            fun H0 H1 =>
+                              (@Delete_Valid _ or Ridx DeletedTuples H0 H1, snd v)
+                          | _, _ => fun _ _ => (or, [])
+                        end H0 H1').
+      econstructor 2 with
+      (comp_a_value := match x as x', x0 as x0'
+                             return decides x' _ ->
+                                    decides x0' _  -> _
+                       with
+                          | true, true =>
+                            fun H0 H1 =>
+                              @Delete_Valid _ or Ridx DeletedTuples H0 H1
+                          | _, _ => fun _ _ => or
+                        end H0 H1').
+      repeat (econstructor; eauto).
+      repeat find_if_inside; try econstructor; simpl in *.
+      unfold GetRelation, Delete_Valid, UpdateUnConstrRelation,
+      UpdateRelation, EnsembleDelete; simpl; split; intros; eauto.
+      rewrite ith_replace_BoundIndex_neq; eauto using string_dec; simpl.
+      rewrite ith_replace_BoundIndex_eq; unfold EnsembleInsert, GetRelation;
+      simpl; intuition.
+      econstructor.
+      econstructor 3 with (v :=  match x as x', x0 as x0'
+                              return decides x' _ ->
+                                     decides x0' _ ->
+                                     _
+                        with
+                          | true, true =>
+                            fun H H0 => (snd v)
+                          | _, _=> fun _ _ => []
+                        end H0 H1').
+      repeat find_if_inside; simpl;
+      try (solve [unfold not; let H := fresh in intros H; eapply NIntup; eapply H;
+      unfold EnsembleInsert; eauto]).
+      simpl in *.
+      destruct_ex; intuition.
+      unfold GetRelation, Delete_Valid, UpdateUnConstrRelation,
+      UpdateRelation, EnsembleDelete; simpl.
+      rewrite ith_replace_BoundIndex_eq; simpl; eauto.
+      repeat apply_in_hyp computes_to_inv; subst; simpl; eauto.
+      eauto using ComplementIntersectionIndexedList.
+      eauto using ComplementIntersectionIndexedList.
+
+      repeat find_if_inside; subst; repeat econstructor.
+
+      simpl.
+      repeat find_if_inside; subst; repeat econstructor.
+      unfold DropQSConstraints, Delete_Valid, EnsembleDelete; simpl.
+      destruct_ex; intuition.
+      repeat apply_in_hyp computes_to_inv; subst; simpl; eauto.
+      unfold GetRelation, Delete_Valid, UpdateUnConstrRelation,
+      UpdateRelation, EnsembleDelete; simpl.
+      unfold GetRelation, Delete_Valid, UpdateUnConstrRelation,
+      UpdateRelation; rewrite imap_replace_BoundedIndex; simpl; eauto using string_dec.
+  Qed.
+
+  Lemma QSDeleteSpec_UnConstr_refine :
+    forall qsSchema (qs : UnConstrQueryStructure qsSchema )
+           (Ridx : @BoundedString (map relName (qschemaSchemas qsSchema)))
+           (DeletedTuples :
+              Ensemble (@Tuple (schemaHeading (QSGetNRelSchema _ Ridx))))
+           (or : QueryStructure qsSchema)
+           refined_schConstr refined_crossConstr,
+      DropQSConstraints_AbsR or qs
+      -> refine {b | decides
+                       b
+                       (forall tup tup',
+                          EnsembleDelete (GetUnConstrRelation qs Ridx) DeletedTuples tup
+                          -> EnsembleDelete (GetUnConstrRelation qs Ridx) DeletedTuples tup'
+                          -> SatisfiesSchemaConstraints Ridx tup tup') }
+                refined_schConstr
+      -> refine ((@Iterate_Decide_Comp _
+                                (fun Ridx' =>
+                                   Ridx' <> Ridx ->
+                                   forall tup',
+                                     (GetUnConstrRelation qs Ridx') tup'
+                                     -> SatisfiesCrossRelationConstraints
+                                        Ridx' Ridx tup'
+                                        (EnsembleDelete (GetUnConstrRelation qs Ridx) DeletedTuples))))
+                refined_crossConstr
+      -> refine
+        (or' <- (qs'       <- Pick (QSDeleteSpec {|qsHint := or |} Ridx DeletedTuples);
+                 deleted   <- Pick (UnIndexedEnsembleListEquivalence
+                                      (Intersection _
+                                                    (GetRelation or Ridx)
+                                                    (Complement _ (GetRelation qs' Ridx))));
+                 ret (qs', deleted));
+         nr' <- {nr' | DropQSConstraints_AbsR (fst or') nr'};
+         ret (nr', snd or'))
+        (schConstr <- refined_schConstr;
+         crossConstr <- refined_crossConstr;
+         match schConstr, crossConstr with
+           | true, true =>
+             deleted   <- Pick (UnIndexedEnsembleListEquivalence
+                                  (Intersection _
+                                                (GetUnConstrRelation qs Ridx)
+                                                (Complement _ (EnsembleDelete (GetUnConstrRelation qs Ridx) DeletedTuples))));
+           ret (UpdateUnConstrRelation qs Ridx (EnsembleDelete (GetUnConstrRelation qs Ridx) DeletedTuples), deleted)
+           | _, _ => ret (qs, [])
+            end).
+  Proof.
+    intros.
+    setoid_rewrite (@QSDeleteSpec_UnConstr_refine' _ qs Ridx).
+    setoid_rewrite <- H0; setoid_rewrite <- H1.
+    repeat (f_equiv; unfold pointwise_relation; intros).
+    unfold DropQSConstraints_AbsR in *; subst.
+    reflexivity.
+  Qed.
+
+  Local Transparent QSDelete.
+
+    Lemma refine_SatisfiesCrossConstraintsDelete
+     : forall (qsSchema : QueryStructureSchema)
+         (qs : UnConstrQueryStructure qsSchema) (Ridx : BoundedString)
+         (DeletedTuples :
+            Ensemble (@Tuple (schemaHeading (QSGetNRelSchema _ Ridx)))),
+       refine
+         (Iterate_Decide_Comp (map relName (qschemaSchemas qsSchema))
+      (fun Ridx' : BoundedIndex (map relName (qschemaSchemas qsSchema)) =>
+       Ridx' <> Ridx ->
+       forall tup' : IndexedTuple,
+       GetUnConstrRelation qs Ridx' tup' ->
+       SatisfiesCrossRelationConstraints Ridx' Ridx tup'
+         (EnsembleDelete (GetUnConstrRelation qs Ridx) DeletedTuples)))
+         (Iterate_Decide_Comp_opt' string
+                          (map relName (qschemaSchemas qsSchema))
+                          []
+                          (fun
+                             Ridx' : BoundedIndex
+                                       ([] ++
+                                        map relName (qschemaSchemas qsSchema)) =>
+                           if BoundedString_eq_dec Ridx Ridx'
+                           then None
+                           else
+                            match
+                              BuildQueryStructureConstraints qsSchema Ridx'
+                                Ridx
+                            with
+                            | Some CrossConstr =>
+                                Some
+                                  (forall tup' : IndexedTuple,
+                                   GetUnConstrRelation qs Ridx' tup' ->
+                                   CrossConstr tup'
+                                     (EnsembleDelete
+                                        (GetUnConstrRelation qs Ridx)
+                                        DeletedTuples))
+                            | None => None
+                            end)).
+    Proof.
+      intros; simpl.
+      setoid_rewrite <- refine_Iterate_Decide_Comp.
+      unfold SatisfiesCrossRelationConstraints.
+      apply refine_Iterate_Decide_Comp_equiv; simpl; intros.
+      apply string_dec.
+      destruct (BoundedString_eq_dec Ridx idx); subst.
+      congruence.
+      destruct (BuildQueryStructureConstraints qsSchema idx Ridx); eauto.
+      intro; eapply H.
+      destruct (BoundedString_eq_dec Ridx idx); subst; eauto.
+      destruct (BuildQueryStructureConstraints qsSchema idx Ridx); eauto.
+    Qed.
+
+    Lemma refine_SatisfiesSchemaConstraintsDelete
+     : forall (qsSchema : QueryStructureSchema)
+         (qs : UnConstrQueryStructure qsSchema) (Ridx : BoundedString)
+         (DeletedTuples :
+            Ensemble (@Tuple (schemaHeading (QSGetNRelSchema _ Ridx)))),
+       refine
+         {b |
+          decides b
+                  (forall tup tup',
+                     EnsembleDelete (GetUnConstrRelation qs Ridx) DeletedTuples tup
+                     -> EnsembleDelete (GetUnConstrRelation qs Ridx) DeletedTuples tup'
+                     -> SatisfiesSchemaConstraints Ridx tup tup') }
+         match schemaConstraints (QSGetNRelSchema qsSchema Ridx) with
+         | Some Constr =>
+           {b | decides
+                  b
+                  (forall tup tup',
+                     EnsembleDelete (GetUnConstrRelation qs Ridx) DeletedTuples tup
+                     -> EnsembleDelete (GetUnConstrRelation qs Ridx) DeletedTuples tup'
+                     -> Constr tup tup') }
+         | None => ret true
+         end.
+    Proof.
+      intros; unfold SatisfiesSchemaConstraints;
+      destruct (schemaConstraints (QSGetNRelSchema qsSchema Ridx)); try reflexivity.
+      intros v Comp_v; econstructor; inversion_by computes_to_inv; subst;
+      simpl; tauto.
+    Qed.
+    
+    
+    Definition QSDeletedTuples
+               qsSchema (qs : UnConstrQueryStructure qsSchema )
+               (Ridx : @BoundedString (map relName (qschemaSchemas qsSchema)))
+               (DeletedTuples :
+                  Ensemble (@Tuple (schemaHeading (QSGetNRelSchema _ Ridx)))) :=
+      (UnIndexedEnsembleListEquivalence
+         (Intersection _
+                       (GetUnConstrRelation qs Ridx)
+                       (Complement _ (EnsembleDelete (GetUnConstrRelation qs Ridx) DeletedTuples)))).
+
+    Lemma QSDeleteSpec_UnConstr_refine_opt :
+      forall qsSchema (qs : UnConstrQueryStructure qsSchema )
+           (Ridx : @BoundedString (map relName (qschemaSchemas qsSchema)))
+           (DeletedTuples :
+              Ensemble (@Tuple (schemaHeading (QSGetNRelSchema _ Ridx))))
+           (or : QueryStructure qsSchema),
+      DropQSConstraints_AbsR or qs ->
+      refine
+        (or' <- (qs'       <- Pick (QSDeleteSpec {|qsHint := or |} Ridx DeletedTuples);
+                 deleted   <- Pick (UnIndexedEnsembleListEquivalence
+                                      (Intersection _
+                                                    (GetRelation or Ridx)
+                                                    (Complement _ (GetRelation qs' Ridx))));
+                 ret (qs', deleted));
+         nr' <- {nr' | DropQSConstraints_AbsR (fst or') nr'};
+         ret (nr', snd or'))
+        match (schemaConstraints (QSGetNRelSchema qsSchema Ridx)) with
+            Some Constr =>
+            schConstr <- {b | decides
+                                b
+                                (forall tup tup',
+                                   EnsembleDelete (GetUnConstrRelation qs Ridx) DeletedTuples tup
+                                   -> EnsembleDelete (GetUnConstrRelation qs Ridx) DeletedTuples tup'
+                                   -> Constr tup tup') };
+              crossConstr <- (@Iterate_Decide_Comp_opt'
+                                _ _ []
+                                (fun Ridx' =>
+                                   if (BoundedString_eq_dec Ridx Ridx') then
+                                     None
+                                   else
+                                     match (BuildQueryStructureConstraints qsSchema Ridx' Ridx) with
+                                       | Some CrossConstr =>
+                                         Some (
+                                             forall tup',
+                                                       (GetUnConstrRelation qs Ridx') tup'
+                                                       -> CrossConstr (indexedTuple tup') (
+                                                                        (EnsembleDelete
+                                                                           (GetUnConstrRelation qs Ridx)
+                                                                           DeletedTuples)))
+                                               | None => None
+                                      end));
+              match schConstr, crossConstr with
+                         | true, true =>
+                           deleted   <- Pick (QSDeletedTuples qs Ridx DeletedTuples);
+                             ret (UpdateUnConstrRelation qs Ridx (EnsembleDelete (GetUnConstrRelation qs Ridx) DeletedTuples), deleted)
+                         | _, _ => ret (qs, [])
+                       end
+          | None =>
+              crossConstr <- (@Iterate_Decide_Comp_opt'
+                                _ _ []
+                                (fun Ridx' =>
+                                   if (BoundedString_eq_dec Ridx Ridx') then
+                                     None
+                                   else
+                                     match (BuildQueryStructureConstraints qsSchema Ridx' Ridx) with
+                                       | Some CrossConstr =>
+                                         Some (
+                                             forall tup',
+                                                       (GetUnConstrRelation qs Ridx') tup'
+                                                       -> CrossConstr (indexedTuple tup') (
+                                                                        (EnsembleDelete
+                                                                           (GetUnConstrRelation qs Ridx)
+                                                                           DeletedTuples)))
+                                               | None => None
+                                      end));
+              match crossConstr with
+                         | true =>
+                           deleted   <- Pick (QSDeletedTuples qs Ridx DeletedTuples);
+                             ret (UpdateUnConstrRelation qs Ridx (EnsembleDelete (GetUnConstrRelation qs Ridx) DeletedTuples), deleted)
+                         | false => ret (qs, [])
+                       end
+        end.
+    Proof.
+      unfold QSDeletedTuples.
+      intros; rewrite QSDeleteSpec_UnConstr_refine;
+      eauto using
+            refine_SatisfiesSchemaConstraintsDelete,
+      refine_SatisfiesCrossConstraintsDelete.
+      destruct (schemaConstraints (QSGetNRelSchema qsSchema Ridx)).
+      reflexivity.
+      simplify with monad laws.
+      f_equiv.
+    Qed.
+
+End DeleteRefinements.
+
+Tactic Notation "remove" "trivial" "deletion" "checks" :=
+  repeat rewrite refineEquiv_bind_bind;
+  etransitivity;
+  [ repeat (apply refine_bind;
+            [reflexivity
+            | match goal with
+                | |- context [Bind (Delete _ from _ where _)%QuerySpec _] =>
+                  unfold pointwise_relation; intros
+                    end
+                 ] );
+    (* Pull out the relation we're inserting into and then
+     rewrite [QSInsertSpec] *)
+    match goal with
+        H : DropQSConstraints_AbsR ?r_o ?r_n
+        |- context [QSDelete ?qs ?R ?P] =>
+          (* If we try to eapply [QSInsertSpec_UnConstr_refine] directly
+                   after we've drilled under a bind, this tactic will fail because
+                   typeclass resolution breaks down. Generalizing and applying gets
+                   around this problem for reasons unknown. *)
+        let H' := fresh in
+        pose proof (@QSDeleteSpec_UnConstr_refine_opt
+                      _ r_n R P r_o H) as H';
+          apply H'
+    end
+  | cbv beta; simpl schemaConstraints; cbv iota;
+    simpl map; simpl app;
+    simpl relName in *; simpl schemaHeading in *;
+    pose_string_ids; simpl;
+    simplify with monad laws;
+    try rewrite <- GetRelDropConstraints;
+    repeat match goal with
+             | H : DropQSConstraints_AbsR ?qs ?uqs |- _ =>
+               rewrite H in *
+           end
+  ].
+
+Tactic Notation "drop" "constraints" "from" "delete" constr(methname) :=
+  hone method methname;
+  [ remove trivial deletion checks;
+    finish honing
+  | ].
