src/QueryStructure/Refinements/OperationRefinements.v
@@ -1,3 +1,3 @@
 Require Export GeneralInsertRefinements GeneralQueryRefinements
         GeneralQueryStructureRefinements ConstraintChecksRefinements
-        ConstraintChecksUnfoldings.
+        ConstraintChecksUnfoldings GeneralDeleteRefinements.
